% mainfile: ../master_thesis_GW.tex
\chapter{Literature summary}
\todo{omówić literaturę}

\section{Coleman Weinberg}\label{CWchapter}
As a founding paper for this conciderations we present:
\todo{zrobić jakieś wprowadzenie}
%\chapter{How did Coleman and Weinberg do it?}
Here, we will present a summary of the parts of \citeColWein that are of interest to us. \\

\section{\texorpdfstring{$\lambda\varphi^4$}{Lambda phi to the fourth} theory}
Coleman and Weinberg in \cite{Coleman1973} start with "$\lambda\varphi^4$" model, namely, with 
Lagransian:
\begin{align}
\mathcal{L} = \frac{1}{2}(\partial_\mu\varphi)^2-\frac{\lambda}{4!}\varphi^4+\frac{1}{2}
A(\partial_\mu\varphi)^2-\frac{1}{2}B\varphi^2-\frac{1}{4!}C\varphi^4,
\end{align}
where $A$, $B$, $C$ are renormalisation constants. \\

Then there are calculations of the renormalised effective potential in this theory. \\

Tree level potential is
\begin{align}
V=\frac{\lambda}{4!}\varphi_c^4,
\end{align}
and up to the one loop level is:
\begin{align}
V = \frac{\lambda}{4!}\varphi_c^4+\frac{1}{2}B\varphi_c^2+\frac{1}{4!}C\varphi_c^4 + 
i\int\frac{d^4k}{(2\pi)^4}\sum\limits_{n=1}^\infty\frac{1}{2n}
\left(\frac{\frac{1}{2}\lambda\varphi_c^2}{k^2+i\epsilon}\right)^n.
\end{align} 
As mentioned in \cite{Coleman1973} and 
\ref{divergent sums}, this expression seems "hideously infrared divergent". It is thus transformed 
into one in Euclidean space with apparent infrared divergence turned into logarithmic 
singularity at $\varphi_c=0$:
\begin{align}
V=\frac{\lambda}{4!}\varphi_c^4+\frac{1}{2}B\varphi_c^2+\frac{1}{4!}C\varphi_c^4 +
\frac{1}{2}\int\frac{d^4k}{(2\pi)^4}\ln\left(1+\frac{\lambda\varphi_c^2}{2k^2}\right).
\end{align}
This is then calculated using cut-off method, with cut off ad $k^2 = \Lambda^2$. 
The result is:
\begin{align}
V=\frac{\lambda}{4!}\varphi_c^4+\frac{1}{2}B\varphi_c^2+\frac{1}{4!}C\varphi_c^4+
\frac{\lambda\Lambda^2}{64\pi^2}\varphi_c^2+\frac{\lambda^2\varphi_c^4}{256\pi^2}
\left(\ln\frac{\lambda\varphi_c^2}{2\Lambda^2}-\frac{1}{2}\right).
\end{align}
\subsection{Renormalisation}
Then, the potential is renormalised. First renormalisation condition is for the 
renormalised mass to vanish (eq. (3.5) in \cite{Coleman1973}). \\

It is written as:
\begin{align}\label{howCW_IIat0}
\frac{d^2V}{d\varphi_c^2}\Big|_0=0.
\end{align}
%This conditin is interesting, as it seems to only postulate  ... \todo{rozwinąć}
%which can be suspitious, as, according to discusion in \cite{Coleman1973} rigth after equation 
%(2.12b), we have that mass is equal to $\frac{d^2V}{d\varphi_c^2}\Big|_{\langle\varphi\rangle}$, 
%where $\langle\varphi\rangle$ is VEV of $\varphi$. \\
%A priori, it is not guaranteed in our theory, that symmetry is unbroken and 
%$\langle\varphi\rangle = 0$. However, it is also not explicitly broken yet, so we left it for now. 
%\\
The second derivative of the potential evaluated at zero is equal to:
\begin{align}
\frac{d^2V}{d\varphi_c^2}\Big|_0 = B+\frac{\lambda\Lambda^2}{32\pi^2},
\end{align}
so condition \ref{howCW_IIat0} gives us, that 
\begin{align}
B = -\frac{\lambda\Lambda^2}{32\pi^2},
\end{align}

Note that, if the derivative would be evaluated at some non zero $\lVEV$, this relation will 
vastly change. \\

We would like to have an analogous condition for the fourth derivative, but
 the fourth derivative does not exist at 0, because of the logarithmic infrared singularity.
To resolve this problem, we can intoduce a prameter $M$, with the dimention of the mass and take 
the derivative at it.
%After determining $B$, the following criterium for determining $C$ is presented:
The condition takes the form:
\begin{align}
\frac{d^4V}{d\varphi_c^4}\Big|_M=\lambda.
\end{align}
%We for now leave (although interesting) discusion of introducing the parameter $M$. \\
%\todo{M parameter }
The parameter $M$ taken is arbitrary. Let us note, that taking different $M'$ will result 
in different $\lambda'$, but the form of the final potential will remain unchanged.\\

The resulting $C$ is:
\begin{align}
C=-\frac{3\lambda^2}{32\pi^2}\left(\ln\frac{\lambda M^2}{2\Lambda^2}+\frac{11}{3}\right).
\end{align}
%Note, that resulting $C$ is completly independent of the value of $B$ determined 
%earlier\label{CBreason}, as $B$ is not present in $\frac{d^4V}{d\varphi_c^4}\Big|_M$. \\
The resulting potential is:
\begin{align}
V=\frac{\lambda}{4!}\varphi_c^4+\frac{\lambda^2\varphi_c^4}{256\pi^2}\left(\ln
\frac{\varphi_c^2}{M^2}-\frac{25}{6}\right).
\end{align}
Then, the discussion proceeds, that, at $\varphi_c = 0$ we have now maximum, not minimum, 
and that the minimum of the potential occurs at the value of: 
$\varphi_c$ determined by:
\begin{align}
\lambda\ln\frac{\lVEV^2}{M^2}=-\frac{32}{3}\pi^2+O(\lambda),
\end{align}
which is very far outside the expected range of validity of the one-loop approximation and must be 
rejected as superficial. \\

%\textit{I am not sure what are the implications of this in physics.}
\section{Scalar electrodynamics}
Now, we will present treatment of the theory of our main interest conducted in 
\cite{Coleman1973}. \\

It starts with the theory with the lagransian \cite{Coleman1973}(4.1):
\begin{align}\label{CW_electrodynamics}
\mathcal{L} = -\frac{1}{4}(F_{\mu\nu})^2+\frac{1}{2}(\partial_\mu\varphi_1-eA_\mu\varphi_2)^2 + 
\frac{1}{2}(\partial_\mu\varphi_2+eA_\mu\varphi_1)^2-\frac{\lambda}{4!}(\varphi_1^2+\varphi_2^2)^2 
 + \textrm{counterterms}.
\end{align}

Then, the resulting renormalised potential is presented \cite{Coleman1973}(4.5):
\begin{align}
V = \frac{\lambda}{4!}\varphi_c^4+\left(\frac{5\lambda^2}{1152\pi^2}+\frac{3e^4}{64\pi^2}\right)
\varphi_c^4\left(\ln\frac{\varphi_c^2}{M^2}-\frac{25}{6}\right),
\end{align}
whith only a brief note, that it is obtained after "straightforward computation" 
%and it is implied that the procedure was the same as in the $\lambda\varphi^4$ case
.\\

We will now investigate more carefully this ommited step
%and whether it was indeed the same as 
%presented in the previous case, as well as, whether this procedure is eligible for this theory.
.\\

It is implied, that the procedure was the same as in the $\lambda\varphi^4$ case and we shall see, 
whether it was indeed the same, as well as, whether applied procedure is eligible for this theory.\\

%Let us go step-by-step through the process. 
Let us start with the effective potential with not yet calculated integrals and not yet evaluated 
renormalisation constants:
\begin{align}
V = &\frac{\lambda}{4!}\varphi_c^4-\frac{1}{2}B\varphi_c^2-\frac{1}{4!}C\varphi_c^4  \notag \\
&+i\int\frac{d^4k}{(2\pi)^4}\sum\limits_{n=1}^\infty\frac{1}{2n}
\left(\frac{\frac{1}{2}\lambda\varphi_c^2}{k^2+i\epsilon}\right)^n  \notag \\
&+i\int\frac{d^4k}{(2\pi)^4}\sum\limits_{n=1}^\infty\frac{1}{2n}
\left(\frac{\frac{1}{6}\lambda\varphi_c^2}{k^2+i\epsilon}\right)^n  \notag \\
&+i\int\frac{d^4k}{(2\pi)^4}3\sum\limits_{n=1}^\infty\frac{1}{2n}
\left(\frac{e^2\varphi_c^2}{k^2+i\epsilon}\right)^n.
\end{align}
This can be transformed as previously from this infrared divergent form, to the form with 
singularity only at $\varphi_c=0$:
\begin{align}
V=&\frac{\lambda}{4!}\varphi_c^4-\frac{1}{2}B\varphi_c^2-\frac{1}{4!}C\varphi_c^4  \notag \\
&+\frac{1}{2}\int\frac{d^4k}{(2\pi)^4}\ln\left(1+\frac{\lambda\varphi_c^2}{2k^2}\right)  \notag \\
&+\frac{1}{2}\int\frac{d^4k}{(2\pi)^4}\ln\left(1+\frac{\lambda\varphi_c^2}{6k^2}\right)  \notag \\
&+\frac{1}{2}\int\frac{d^4k}{(2\pi)^4}3\ln\left(1+\frac{e^2\varphi_c^2}{k^2}\right),
\end{align}
and then calculated using cut-off method at $k^2=\Lambda^2$:
\begin{align}
V=&\frac{\lambda}{4!}\varphi_c^4+\frac{1}{2}B\varphi_c^2+\frac{1}{4!}C\varphi_c^4 \notag \\
&+\frac{\lambda\Lambda^2}{64\pi^2}\varphi_c^2+\frac{\lambda^2\varphi_c^4}{256\pi^2}
\left(\ln\frac{\lambda\varphi_c^2}{2\Lambda^2}-\frac{1}{2}\right)  \notag \\
&+\frac{\lambda\Lambda^2}{3\cdot 64\pi^2}\varphi_c^2+\frac{\lambda^2\varphi_c^4}{9\cdot 256\pi^2}
\left(\ln\frac{\lambda\varphi_c^2}{6\Lambda^2}-\frac{1}{2}\right)  \notag \\
&+\frac{3e^2\Lambda^2}{32\pi^2}\varphi_c^2+\frac{3e^4\varphi_c^4}{64\pi^2}
\left(\ln\frac{e^2\varphi_c^2}{\Lambda^2}-\frac{1}{2}\right).
\end{align}
%where $\alpha$ is some numerical constant.

\subsection{Renormalisation}\label{CW_renormalisation_scalar_el}
%Now, it starts the fun part. \\
The first imposed renormalisation condition in the previous ($\lambda\varphi^4$) case was:
\begin{align}\label{phitoforth condition}
\frac{d^2V}{d\varphi_c^2}\Big|_0=0,
\end{align}
where, it was stated, is equivalent, to renormalised mass being zero. \\

What is important, this "renormalized mass" is not meant to be a physicall mass, rather, 
the mass parameter, the constant that stand beside second power of the field, 
which can be defined as "$\frac{d^2V}{d\varphi_c^2}\Big|_0$" itself. \\

%But it is only true, when $\lVEV = 0$. In theory we are discussing now (\ref{CW_electrodynamics}) 
%we can't really use this as (as it is made apparent later in \cite{Coleman1973}, in (4.8)), the 
%whole important later argument is laid upon the fact, that $\lVEV \neq 0$. It also can't be, that 
%we are now dealing with tree level VEV, which is $0$, and after that, we pass to using on-loop 
%level VEV which is non-zero, as the very VEV used in the renormalised condition, should be one 
%of the up to one loop level potential -- thus renormalised one. Or can we? Maybe we can use 
%zero $\lVEV$ now, and not zero $\lVEV$ later. Nevertheless, 
%Here it is not explicitly stated, whether this condition is being used in the case of scalar 
%electrodynamics and we shall investigate that matter. \\
%, whether this is the case, and whether this was used here. \\
The same renormalisation condition was used as the first one in this case. \\

The second derivative evaluated at zero is:
\begin{align}
\frac{d^2V}{d\varphi_c^2}\Big|_0 = 
\frac{1}{2}B\varphi_c^2 + 
\frac{\lambda\Lambda^2}{64\pi^2}\varphi_c^2+ 
\frac{\lambda\Lambda^2}{3\cdot 64\pi^2}\varphi_c^2+
\frac{3e^2\Lambda^2}{32\pi^2}\varphi_c^2. 
\end{align}
Thus:
\begin{align}\label{CW_B_dm}
B = -2\Big(
\frac{\lambda\Lambda^2}{64\pi^2}+ 
\frac{\lambda\Lambda^2}{3\cdot 64\pi^2}+
\frac{3e^2\Lambda^2}{32\pi^2}\Big). 
\end{align}
The second renormalisation condition is:
%Let us start with the second renormalisation condition, namely:
\begin{align}
\frac{d^4V}{d\varphi_c^4}\Big|_M=\lambda,
\end{align}
%and reverse engeneer what happened in \cite{Coleman1973}. \\
%We can do this, because of the reason stated in \ref{CBreason} as $B$ does not appear in 
%$\frac{d^4V}{d\varphi_c^4}\Big|_M$. \\
We have that:
\begin{align}
\frac{d^4V}{d\varphi_c^4}\Big|_M = &\lambda + C \notag \\
&+\frac{11\lambda^2}{32\pi^2}+\frac{3\lambda^2}{32\pi^2}\ln\frac{\lambda M^2}{2\Lambda^2}\notag \\
&+\frac{11\lambda^2}{288\pi^2}+\frac{\lambda^2}{96\pi^2}\ln\frac{\lambda M^2}{6\Lambda^2}\notag \\
&+\frac{(75-18\alpha)e^4}{16\pi^2}+\frac{9e^4}{8\pi^2}\ln\frac{e^2M^2}{\Lambda^2}. 
\end{align}
From this, for $\frac{d^4V}{d\varphi_c^4}\Big|_M=\lambda$, we conclude that:
\begin{align}
C = -\Big(
&\frac{11\lambda^2}{32\pi^2}+\frac{3\lambda^2}{32\pi^2}\ln\frac{\lambda M^2}{2\Lambda^2}\notag \\
&+\frac{11\lambda^2}{288\pi^2}+\frac{\lambda^2}{96\pi^2}\ln\frac{\lambda M^2}{6\Lambda^2}\notag \\
&+\frac{(75-18\alpha)e^4}{16\pi^2}+\frac{9e^4}{8\pi^2}\ln\frac{e^2M^2}{\Lambda^2}
\Big).
\end{align}
Subsituing these results to the potential result in:
\begin{align}
V=&\frac{\lambda}{4!}\varphi_c^4-\Big(
\frac{\lambda\Lambda^2}{64\pi^2}+ 
\frac{\lambda\Lambda^2}{3\cdot 64\pi^2}+
\frac{3e^2\Lambda^2}{32\pi^2}\Big)\varphi_c^2 \notag \\
&-\frac{1}{4!}\Big(
\frac{11\lambda^2}{32\pi^2}+\frac{3\lambda^2}{32\pi^2}\ln\frac{\lambda M^2}{2\Lambda^2}\notag \\
&+\frac{11\lambda^2}{288\pi^2}+\frac{\lambda^2}{96\pi^2}\ln\frac{\lambda M^2}{6\Lambda^2}\notag \\
&+\frac{(75-18\alpha)e^4}{16\pi^2}+\frac{9e^4}{8\pi^2}\ln\frac{e^2M^2}{\Lambda^2}
\Big)\varphi_c^4 \notag \\
&+\frac{\lambda\Lambda^2}{64\pi^2}\varphi_c^2+\frac{\lambda^2\varphi_c^4}{256\pi^2}
\left(\ln\frac{\lambda\varphi_c^2}{2\Lambda^2}-\frac{1}{2}\right)  \notag \\
&+\frac{\lambda\Lambda^2}{3\cdot 64\pi^2}\varphi_c^2+\frac{\lambda^2\varphi_c^4}{9\cdot 256\pi^2}
\left(\ln\frac{\lambda\varphi_c^2}{6\Lambda^2}-\frac{1}{2}\right)  \notag \\
&+\frac{3e^2\Lambda^2}{32\pi^2}\varphi_c^2+\frac{3e^4\varphi_c^4}{64\pi^2}
\left(\ln\frac{e^2\varphi_c^2}{\Lambda^2}-\frac{1}{2}\right),
\end{align}
and after canceling the renormalised potential is indeed:
\begin{align}
V = &\frac{\lambda}{4!}\varphi_c^4
+\left(\frac{5\lambda^2}{1152\pi^2}+\frac{3e^4}{64\pi^2}\right)\varphi_c^4
\left(\ln\frac{\varphi_c^2}{M^2}-\frac{25}{6}\right).
\end{align}
%%Let us notice, that the constant $\alpha$ disappeared entearly from the expression as it was 
%%canceld out. \\
%Let us notice, that above potential differs from \cite{Coleman1973}(4.5) only by the terms:
%\begin{align}
%\frac{1}{2}B\varphi_c^2 + 
%\frac{\lambda\Lambda^2}{64\pi^2}\varphi_c^2+ 
%\frac{\lambda\Lambda^2}{3\cdot 64\pi^2}\varphi_c^2+
%\frac{3e^2\Lambda^2}{32\pi^2}\varphi_c^2. 
%\end{align}
%As such, in the renormalistion scheme used in \cite{Coleman1973}, we must have that:
%\begin{align}
%\frac{1}{2}B\varphi_c^2 + 
%\frac{\lambda\Lambda^2}{64\pi^2}\varphi_c^2+ 
%\frac{\lambda\Lambda^2}{3\cdot 64\pi^2}\varphi_c^2+
%\frac{3e^2\Lambda^2}{32\pi^2}\varphi_c^2 = 0, 
%\end{align}
%thus:
%\begin{align}\label{CW_B_dm}
%B = -2\Big(
%\frac{\lambda\Lambda^2}{64\pi^2}+ 
%\frac{\lambda\Lambda^2}{3\cdot 64\pi^2}+
%\frac{3e^2\Lambda^2}{32\pi^2}\Big). 
%\end{align}
%Then, the renormalised potential is indeed:
%\begin{align}
%V = \frac{\lambda}{4!}\varphi_c^4+
%\left(\frac{5\lambda^2}{1152\pi^2}+\frac{3e^4}{64\pi^2}\right)\varphi_c^4
%\left(\ln\frac{\varphi_c^2}{M^2}-\frac{25}{6}\right)
%\end{align}
%as in \cite{Coleman1973}(4.5), but what is important is, then indeed
%\begin{align}
%\frac{d^2V}{d\varphi_c^2}\Big|_0=0,
%\end{align}
%so this was preceisly the condition used to renormalised this potential. \\
%Now this is the mystery: \\
%This condition, in the light of this theory, should not mean the disapperance of the renormalised 
%mass, as $\lVEV \neq 0$ in this theory, and the mass is $\frac{d^2V}{d\varphi_c^2}\Big|_\lVEV$. 
%As such, what physical meaning this condition gives? 
%From the computational point of view, it certainly results in the potential being of order $4$ 
%in the field, but physical one? \\
%In \ref{onshellphi4} we will investigate the on-shell approuch of this method.
Let us note, that 
\ref{phitoforth condition}
is precesuily the condition, that guarantees the $\varphi^4$ form of the potential.
%\todo{Napisać o stosunku mas}
\label{CWe4potential}
\subsection{The mass ratio}
The parameter $M$ taken was arbitrary, so we can as well set it to $\langle\varphi\rangle$.
Then, the potentail takes form: 
\begin{align}
V = &\frac{\lambda}{4!}\varphi_c^4
+\left(\frac{5\lambda^2}{1152\pi^2}+\frac{3e^4}{64\pi^2}\right)\varphi_c^4
\left(\ln\frac{\varphi_c^2}{\langle\varphi\rangle^2}-\frac{25}{6}\right). 
\end{align} 
As $\langle\varphi\rangle$ is defined to be the minimum of the potential, we have that:
\begin{align}
\frac{dV}{d\varphi_c}\Big|_{\langle\varphi\rangle} = 0.
\end{align} 
Thus:
\begin{align}
\left(\frac{\lambda}{6}-\frac{11e^4}{16\pi^2}\right)\langle\varphi\rangle^3 = 0.
\end{align}
The actual location of the minimum is non-zero, so:
\begin{align}
\lambda = \frac{33}{8\pi^2}e^4.
\end{align}
From this, we can rewrite potential as:
\begin{align}\label{CW_e_phi_potential}
V = \frac{3e^4}{64\pi^2}\varphi^4\left(\ln{\frac{\varphi^2}{\langle\varphi\rangle^2}-
\frac{1}{2}}\right).
\end{align}
This gives parametrisation of potential with $e$ and $\langle\varphi\rangle$ alone. 
With different $M$ choosen, the $\lambda$ would change and intermediate expressions would change, 
but \ref{CW_e_phi_potential} would remain the same.
From this we can express masses of the scalar and the vector in terms of $e$ and $\varphi$.
The mass of the scalar is:
\begin{equation}
m^2(S) = \frac{d^2V}{d\varphi_c^2}\Big|_{\langle\varphi\rangle} = 
\frac{3e^4}{8\pi^2}\langle\varphi\rangle^2.
\end{equation}
The mass of the vector is:
\begin{equation}
m^2(V) = e^2\frac{d^2V}{d\varphi_c^2}\Big|_0.
\end{equation}
From this, the mass ratio is obtained:
\begin{equation}
\frac{m^2(S)}{m^2(V)} = \frac{3}{2\pi}\frac{e^2}{4\pi} = \frac{3e^2}{8\pi^2}.
\end{equation}


\todo{napisać koniecznie o radiacyjnym łamaniu symetrii w tym rozdziale}
\todo{napisać o tym jak to oni biorą tą pochodną w zerze}

\section{Possible approuches}

\todo{wprowadzenie do tego, co my chcemy zrobić}

















